AxiomaticModels/GenAxiomaticArm.v
@@ -1,0 +1,1314 @@
+Require Import Strings.String.
+
+From stdpp Require Import decidable.
+
+Require Import SSCCommon.Common.
+Require Import SSCCommon.GRel.
+Require Import SSCCommon.FMon.
+Require Import ISASem.ArmInst.
+Require Import ISASem.SailArmInstTypes.
+Require Import GenModels.TermModels.
+Module ArmTM := TermModels Arm.
+Require Import GenModels.CandidateExecutions.
+Module ArmCand := CandidateExecutions Arm ArmTM.
+
+Import Arm.
+Import ArmTM.
+Import ArmCand.
+
+(* NOTE:
+ This file defines the VMSA and User Arm axiomatic models. It starts with some
+ common definitions (in section common_def), followed by module GenArm which
+ contains a candidate cd, an inital memory map init_mem, with preliminary common
+ wellformedness conditions. Finally, the two modules VMSA and UM contain the two
+ models and their specific wellformedness conditions respectively. There are no
+ dependencies between the two models.
+ *)
+
+Section common_def.
+  Import Candidate.
+
+  #[local] Hint Extern 10 (Decision (?x _)) => unfold x : typeclass_instances.
+  #[local] Hint Extern 10 (Decision (?x _ _)) => unfold x : typeclass_instances.
+  #[local] Hint Extern 10 (Decision (?x _ _ _)) => unfold x : typeclass_instances.
+
+  (*** barriers *)
+  (* armv9-interface/barriers.cat *)
+  Implicit Type b : SailArmInstTypes.Barrier.
+
+  Definition is_barrier_P P `{forall b, Decision (P b)} (event : iEvent) :=
+    match event with
+    | Barrier b &→ _ => P b
+    | _ => False
+    end.
+
+  Global Instance is_barrier_P_dec P `{forall b, Decision (P b)} event :
+    Decision (is_barrier_P P event).
+  Proof. apply _. Qed.
+
+  Definition is_isb (barrier : barrier) :=
+    match barrier with
+    | Barrier_ISB _ => True
+    | _ => False
+    end.
+
+  Definition isb {n} (cd : Candidate.t n) :=
+    collect_all (λ _ event, is_barrier_P is_isb event) cd.
+
+  Definition has_dsb_P P `{forall dxb, Decision (P dxb)} (barrier : barrier) :=
+    match barrier with
+    | Barrier_DSB dxb => P dxb
+    | _ => False
+    end.
+
+  Global Instance has_dsb_P_dec P `{forall dxb, Decision (P dxb)} barrier :
+    Decision (has_dsb_P P barrier).
+  Proof. apply _. Qed.
+
+  Definition is_dsbsy := has_dsb_P
+                           (λ dxb,
+                              (* DSBISH *)
+                              (dxb.(DxB_domain) = MBReqDomain_InnerShareable
+                               ∧ dxb.(DxB_types) = MBReqTypes_All)
+                              (* DSBSY *)
+                              ∨ (dxb.(DxB_domain) = MBReqDomain_FullSystem
+                                 ∧ dxb.(DxB_types) = MBReqTypes_All)
+                              (* DSBNSH *)
+                              ∨ (dxb.(DxB_domain) = MBReqDomain_Nonshareable
+                                 ∧ dxb.(DxB_types) = MBReqTypes_All)
+                           ).
+
+  Global Instance is_dsbsy_dec dxb : Decision (is_dsbsy dxb).
+  Proof. apply _. Qed.
+
+  (* armv9-interface/barriers.cat#L112 *)
+  Definition dsbsy {n} (cd : Candidate.t n) :=
+    collect_all (λ _ event, is_barrier_P is_dsbsy event) cd.
+
+  Definition is_dsbst b := is_dsbsy b
+                           ∨ (has_dsb_P
+                                (λ dxb,
+                                   (* DSBST *)
+                                   (dxb.(DxB_types) = MBReqTypes_Writes)
+                                   (* DSBISHST *)
+                                   ∨ (dxb.(DxB_domain) = MBReqDomain_InnerShareable
+                                      ∧ dxb.(DxB_types) = MBReqTypes_Writes)
+                                   (* DSBNSHST *)
+                                   ∨ (dxb.(DxB_domain) = MBReqDomain_Nonshareable
+                                      ∧ dxb.(DxB_types) = MBReqTypes_Writes)
+                                ) b).
+
+  Global Instance is_dsbst_dec dxb : Decision (is_dsbst dxb).
+  Proof. apply _. Qed.
+
+  (* armv9-interface/barriers.cat#L115 *)
+  Definition dsbst {n} (cd : Candidate.t n) :=
+    collect_all (λ _ event, is_barrier_P is_dsbst event) cd.
+
+  Definition is_dsbld b := is_dsbsy b
+                           ∨ (has_dsb_P
+                                (λ dxb,
+                                   (* DSBLD *)
+                                   (dxb.(DxB_types) = MBReqTypes_Reads)
+                                   (* DSBISHLD *)
+                                   ∨ (dxb.(DxB_domain) = MBReqDomain_InnerShareable
+                                      ∧ dxb.(DxB_types) = MBReqTypes_Reads)
+                                   (* DSBNSHLD *)
+                                   ∨ (dxb.(DxB_domain) = MBReqDomain_Nonshareable
+                                      ∧ dxb.(DxB_types) = MBReqTypes_Reads)
+                                ) b).
+
+  Global Instance is_dsbld_dec dxb : Decision (is_dsbld dxb).
+  Proof. apply _. Qed.
+
+  (* armv9-interface/barriers.cat#L115 *)
+  Definition dsbld {n} (cd : Candidate.t n) :=
+    collect_all (λ _ event, is_barrier_P is_dsbld event) cd.
+
+  Definition is_dsbnsh := has_dsb_P
+                            (λ dxb,
+                               (* DSBNSH *)
+                               (dxb.(DxB_domain) = MBReqDomain_InnerShareable
+                                ∧ dxb.(DxB_types) = MBReqTypes_All)).
+
+  Global Instance is_dsbnsh_dec dxb : Decision (is_dsbnsh dxb).
+  Proof. apply _. Qed.
+
+  (* armv9-interface/barriers.cat#L121 *)
+  Definition dsbnsh {n} (cd : Candidate.t n) :=
+    collect_all (λ _ event, is_barrier_P is_dsbnsh event) cd.
+
+
+  Definition has_dmb_P P `{forall dxb, Decision (P dxb)} (barrier : barrier) :=
+    match barrier with
+    | Barrier_DMB dxb => P dxb
+    | _ => False
+    end.
+
+  Global Instance has_dmb_P_dec P `{forall dxb, Decision (P dxb)} barrier :
+    Decision (has_dmb_P P barrier).
+  Proof. apply _. Qed.
+
+  Definition is_dmbsy b := is_dsbsy b
+                           ∨ (has_dmb_P
+                                (λ dxb,
+                                   (* DMBSY *)
+                                   (dxb.(DxB_domain) = MBReqDomain_FullSystem
+                                    ∧ dxb.(DxB_types) = MBReqTypes_All)
+                                   (* DMBISH *)
+                                   ∨ (dxb.(DxB_domain) = MBReqDomain_InnerShareable
+                                      ∧ dxb.(DxB_types) = MBReqTypes_All)
+                                   (* DMBNSH *)
+                                   ∨ (dxb.(DxB_domain) = MBReqDomain_Nonshareable
+                                      ∧ dxb.(DxB_types) = MBReqTypes_All)
+                                ) b).
+
+  Global Instance is_dmbsy_dec dxb : Decision (is_dmbsy dxb).
+  Proof. apply _. Qed.
+
+  (* armv9-interface/barriers.cat#L124 *)
+  Definition dmbsy {n} (cd : Candidate.t n) :=
+    collect_all (λ _ event, is_barrier_P is_dmbsy event) cd.
+
+  Definition is_dmbst b := is_dmbsy b ∨ is_dsbst b
+                           ∨ (has_dmb_P
+                                (λ dxb,
+                                   (* DMBST *)
+                                   (dxb.(DxB_domain) = MBReqDomain_FullSystem
+                                    ∧ dxb.(DxB_types) = MBReqTypes_Writes)
+                                   (* DMBISHST *)
+                                   ∨ (dxb.(DxB_domain) = MBReqDomain_InnerShareable
+                                      ∧ dxb.(DxB_types) = MBReqTypes_Writes)
+                                   (* DMBNSHST *)
+                                   ∨ (dxb.(DxB_domain) = MBReqDomain_Nonshareable
+                                      ∧ dxb.(DxB_types) = MBReqTypes_Writes)
+                                ) b).
+
+  Global Instance is_dmbst_dec dxb : Decision (is_dmbst dxb).
+  Proof. apply _. Qed.
+
+  (* armv9-interface/barriers.cat#L127 *)
+  Definition dmbst {n} (cd : Candidate.t n) :=
+    collect_all (λ _ event, is_barrier_P is_dmbst event) cd.
+
+  Definition is_dmbld b := is_dmbsy b ∨ is_dsbld b
+                           ∨ (has_dmb_P
+                                (λ dxb,
+                                   (* DMBLD *)
+                                   (dxb.(DxB_domain) = MBReqDomain_FullSystem
+                                    ∧ dxb.(DxB_types) = MBReqTypes_Reads)
+                                   (* DMBISHLD *)
+                                   ∨ (dxb.(DxB_domain) = MBReqDomain_InnerShareable
+                                      ∧ dxb.(DxB_types) = MBReqTypes_Reads)
+                                   (* DMBNSHLD *)
+                                   ∨ (dxb.(DxB_domain) = MBReqDomain_Nonshareable
+                                      ∧ dxb.(DxB_types) = MBReqTypes_Reads)
+                                ) b).
+
+  Global Instance is_dmbld_dec dxb : Decision (is_dmbld dxb).
+  Proof. apply _. Qed.
+
+  (* armv9-interface/barriers.cat#L130 *)
+  Definition dmbld {n} (cd : Candidate.t n) :=
+    collect_all (λ _ event, is_barrier_P is_dmbld event) cd.
+
+  Definition is_dmb b := is_dmbsy b ∨ is_dmbst b ∨ is_dmbld b.
+
+  Global Instance is_dmb_dec dxb : Decision (is_dmb dxb).
+  Proof. apply _. Qed.
+
+  (* armv9-interface/barriers.cat#L133 *)
+  Definition dmb {n} (cd : Candidate.t n) :=
+    collect_all (λ _ event, is_barrier_P is_dmb event) cd.
+
+  Definition is_dsb b := is_dsbsy b ∨ is_dsbst b ∨ is_dsbld b.
+
+  Global Instance is_dsb_dec dxb : Decision (is_dsb dxb).
+  Proof. apply _. Qed.
+
+  (* armv9-interface/barriers.cat#L136 *)
+  Definition dsb {n} (cd : Candidate.t n) :=
+    collect_all (λ _ event, is_barrier_P is_dsb event) cd.
+
+
+  Definition is_explicit_access_kind_P P (event : iEvent) : Prop :=
+    match event with
+    | MemRead _ rreq &→ _ => match rreq.(ReadReq.access_kind) with
+                                  | AK_explicit ak => P ak
+                                  | _ => False
+                                  end
+    | MemWrite _ wreq &→ _ => match wreq.(WriteReq.access_kind) with
+                                   | AK_explicit ak => P ak
+                                   | _ => False
+                                   end
+    | _ => False
+    end.
+
+  Context {nmth : nat}.
+  Context `(cd : t nmth).
+
+  (*** interface-common *)
+
+  (* interface-common.cat#L2 *)
+  Definition F := barriers cd.
+
+  (* interface-common.cat#L6 *)
+  (* explicit writes *)
+  Definition W :=
+    collect_all (λ _ event, is_mem_write event
+                            ∧ is_explicit_access_kind_P (λ _, True) event) cd.
+
+  (* interface-common.cat#L5 *)
+  Definition R :=
+    collect_all (λ _ event, is_mem_read event
+                            ∧ is_explicit_access_kind_P (λ _, True) event) cd.
+
+  (* interface-common.cat#L52 *)
+  Definition L :=
+    collect_all
+      (λ _ event, is_mem_write event
+                  ∧ is_explicit_access_kind_P
+                      (λ ak, ak.(Explicit_access_kind_strength) = AS_rel_or_acq)
+                      event) cd.
+
+  (* interface-common.cat#L46 *)
+  Definition A :=
+    collect_all
+      (λ _ event, is_mem_read event
+                  ∧ is_explicit_access_kind_P
+                      (λ ak, ak.(Explicit_access_kind_strength) = AS_rel_or_acq)
+                      event) cd.
+
+  (* interface-common.cat#L49 *)
+  Definition Q :=
+    collect_all
+      (λ _ event, is_mem_read event
+                  ∧ is_explicit_access_kind_P
+                      (λ ak, ak.(Explicit_access_kind_strength) = AS_acq_rcpc)
+                      event) cd.
+
+  Definition is_tlbi (event : iEvent) :=
+    match event with
+    | TlbOp _ _ &→ _ => True
+    | _ => False
+    end.
+
+  Global Instance is_tlbi_dec event : Decision (is_tlbi event).
+  Proof. apply _. Qed.
+
+  Definition is_cacheop (event : iEvent) :=
+    match event with
+    | CacheOp _ _ &→ _ => True
+    | _ => False
+    end.
+
+  Global Instance is_cacheop_dec event : Decision (is_cacheop event).
+  Proof. unfold is_cacheop. apply _. Qed.
+
+  (* interface-common.cat#L65 *)
+  Definition C := collect_all (λ _ event, is_tlbi event ∨ is_cacheop event) cd.
+
+  (* interface-common.cat#L68 *)
+  Definition TLBI := collect_all (λ _ event, is_tlbi event) cd.
+
+  Definition is_take_exception (event : iEvent) :=
+    match event with
+    | TakeException _ &→ _ => True
+    | _ => False
+    end.
+
+  Global Instance is_take_exception_dec event : Decision (is_take_exception event).
+  Proof. apply _. Qed.
+
+  (* interface-common.cat#L71 *)
+  Definition TE := collect_all (λ _ event, is_take_exception event) cd.
+
+  Definition is_return_exception (event : iEvent) :=
+    match event with
+    | ReturnException _ &→ _ => True
+    | _ => False
+    end.
+
+  Global Instance is_return_exception_dec event :
+    Decision (is_return_exception event).
+  Proof. apply _. Qed.
+
+  (* interface-common.cat#L72 *)
+  Definition ERET := collect_all (λ _ event, is_return_exception event) cd.
+
+  (*** regs *)
+
+  (* armv9-interface/regs.cat#L2 *)
+  Definition is_msr (event : iEvent) :=
+    match event with
+    | RegWrite _ (Some _) _ _ &→ _ => True
+    | _ => False
+  end.
+  Global Instance is_msr_dec event : Decision (is_msr event).
+  Proof. unfold is_msr. apply _. Qed.
+
+  Definition MSR := collect_all (λ _ event, is_msr event) cd.
+
+  (* translation-table-walk reads *)
+  Definition is_translate (event : iEvent) :=
+    match event with
+    | MemRead _ rreq &→ _ => rreq.(ReadReq.access_kind) = AK_ttw ()
+    | _ => False
+    end.
+
+  Global Instance is_translate_dec event : Decision (is_translate event).
+  Proof. apply _. Qed.
+
+  (* translation-common.cat#L9 *)
+  Definition T := collect_all (λ _ event, is_translate event) cd.
+
+  (* A MemRead with ttw and value 0 *)
+  Definition is_translation_read_fault (event : iEvent) :=
+    match event with
+    | MemRead n rreq &→ resp =>
+        match rreq.(ReadReq.access_kind), resp with
+        | AK_ttw (), inl (val, _) => val = bv_0 _
+        | _, _ => False
+        end
+    | _ => False
+    end.
+
+  Global Instance is_translation_fault_dec event :
+    Decision (is_translation_read_fault event).
+  Proof.
+    unfold is_translation_read_fault.
+    destruct event as [T call ret].
+    destruct call; tc_solve.
+  Qed.
+
+  (* translation-common.cat#L10 *)
+  Definition T_f := collect_all (λ _ event, is_translation_read_fault event) cd.
+
+  Notation "'lxsx'" := (lxsx cd).
+  Notation "'amo'" := (amo cd).
+  Notation "'addr'" := (addr cd).
+  Notation "'data'" := (data cd).
+  Notation "'ctrl'" := (ctrl cd).
+  Notation "'loc'" := (loc cd).
+  (* all mem events (explicit and translation) *)
+  Notation "'writes'" := (mem_writes cd).
+  (* all mem events (explicit and translation) *)
+  Notation "'reads'" := (mem_reads cd).
+
+  (* will diverge from loc if merging events *)
+  Definition overlap_loc := loc.
+
+  Definition rmw := lxsx ∪ amo.
+
+  (* translation-common.cat#L25 *)
+  Notation "'iio'" := (iio cd).
+  (* instruction_order orders events between instructions *)
+  (* translation-common.cat#L26 *)
+  Notation "'instruction_order'" := (instruction_order cd).
+
+End common_def.
+
+Module GenArm.
+  Import Candidate.
+  Section def.
+    Context {nmth : nat}.
+    Context (cd : Candidate.t nmth).
+
+  Notation "'amo'" := (amo cd).
+  Notation "'lxsx'" := (lxsx cd).
+  Notation "'iio'" := (iio cd).
+  Notation "'loc'" := (loc cd).
+  Notation "'addr'" := (addr cd).
+  Notation "'data'" := (data cd).
+  Notation "'ctrl'" := (ctrl cd).
+  Notation "'instruction_order'" := (instruction_order cd).
+  Notation "'W'" := (W cd).
+  Notation "'R'" := (R cd).
+
+  Global Instance is_explicit_access_kind_dec P `{forall ak, Decision (P ak)} event :
+    Decision (is_explicit_access_kind_P P event).
+  Proof. unfold is_explicit_access_kind_P. apply _. Qed.
+
+  Definition is_successful (event : iEvent) :=
+    match event with
+    | MemWrite _ _ &→ wresp =>
+        match wresp with (inl (Some true)) | (inl None) => True | _ => False end
+    | _ => False
+    end.
+
+  Global Instance is_successful_dec event : Decision (is_successful event).
+  Proof.
+    unfold is_successful.
+    destruct event as [T call ret].
+    destruct call; apply _.
+  Qed.
+
+  Definition Wx :=
+    collect_all
+      (λ _ event, is_mem_write event ∧ is_successful event
+                  ∧ is_explicit_access_kind_P
+                      (λ ak, ak.(Explicit_access_kind_variety) = AV_exclusive)
+                      event) cd.
+
+  Definition Rx :=
+    collect_all
+      (λ _ event, is_mem_read event
+                  ∧ is_explicit_access_kind_P
+                      (λ ak, ak.(Explicit_access_kind_variety) = AV_exclusive)
+                      event) cd.
+
+  Export NMSWF.
+
+  Record amo_wf := {
+      amo_dom : grel_dom amo ⊆ Rx;
+      amo_rng : grel_rng amo ⊆ Wx;
+      amo_in_iio : amo ⊆ iio;
+      amo_func : grel_functional amo;
+      amo_inv_func : grel_functional (amo⁻¹);
+      amo_loc : amo ⊆ loc;
+    }.
+
+  Record lxsx_wf := {
+      lxsx_dom : grel_dom lxsx ⊆ Rx;
+      lxsx_rng : grel_rng lxsx ⊆ Wx;
+      lxsx_func : grel_functional lxsx;
+      lxsx_inv_func : grel_functional (lxsx⁻¹);
+      lxsx_loc : lxsx ⊆ loc;
+      lxsx_po : lxsx ⊆ instruction_order;
+    }.
+
+  Record addr_wf :=
+    {
+      addr_dom : grel_dom addr ⊆ R;
+      addr_rng : grel_rng addr ⊆ R ∪ W;
+      addr_in_instruction_order : addr ⊆ instruction_order;
+    }.
+
+  Record data_wf :=
+    {
+      data_dom : grel_dom data ⊆ R;
+      data_rng : grel_rng data ⊆ W;
+      data_in_instruction_order : data ⊆ instruction_order;
+    }.
+
+  Record ctrl_wf :=
+    {
+      ctrl_dom : grel_dom ctrl ⊆ R;
+      ctrl_in_instruction_order : ctrl ⊆ instruction_order;
+      ctrl_instruction_order_in_ctrl : ctrl⨾instruction_order ⊆ ctrl;
+    }.
+
+  Record wellformed:= {
+      amo :> amo_wf;
+      lxsx :> lxsx_wf;
+      generic_po :> NMSWF.generic_po_wf' cd;
+      addr :> addr_wf;
+      data :> data_wf;
+      ctrl :> ctrl_wf;
+    }.
+
+  (* from promising *)
+  Definition get_init_val (a : pa) (init_mem : memoryMap) :=
+    list_from_func 8
+      (fun n => a |> set FullAddress_address (bv_add (Z_to_bv 52 (Z.of_nat n))))
+      |> map init_mem |> bv_of_bytes 64.
+
+  Definition is_initial event init_mem :=
+    (match Candidate.get_pa event, NMSWF.get_val event with
+     | Some pa, Some val => (get_init_val pa init_mem) = val
+     | _, _ => False
+     end).
+
+  Global Instance is_initial_dec event init_mem :
+    Decision (is_initial event init_mem).
+  Proof. unfold is_initial. apply _. Qed.
+
+  End def.
+
+  Variable nmth : nat.
+  Variable cd : Candidate.t nmth.
+  Variable init_mem : memoryMap.
+
+End GenArm.
+
+
+(*** VMSA *)
+Module VMSA.
+  (*** aarch64_mmu_strong_ETS *)
+  Section def.
+    Context {nmth : nat}.
+    Context `(cd : Candidate.t nmth).
+
+    Import Candidate.
+
+    Notation "'W'" := (W cd).
+    Notation "'R'" := (R cd).
+    Notation "'A'" := (A cd).
+    Notation "'Q'" := (Q cd).
+    Notation "'L'" := (L cd).
+    Notation "'F'" := (F cd).
+    Notation "'C'" := (C cd).
+    Notation "'M'" := (W ∪ R).
+    Notation "'T'" := (T cd).
+    Notation "'T_f'" := (T_f cd).
+    Notation "'TLBI'" := (TLBI cd).
+    Notation "'MSR'" := (MSR cd).
+    Notation "'TE'" := (TE cd).
+    Notation "'ERET'" := (ERET cd).
+    Notation "'ISB'" := (isb cd).
+
+    Notation "'rmw'" := (rmw cd).
+    Notation "'addr'" := (addr cd).
+    Notation "'data'" := (data cd).
+    Notation "'ctrl'" := (ctrl cd).
+    Notation "'loc'" := (loc cd).
+    Notation "'int'" := (int cd).
+    Notation "'iio'" := (iio cd).
+
+    Notation "'instruction_order'" := (instruction_order cd).
+    Notation "'overlap_loc'" := (overlap_loc cd).
+
+    Notation "'dmbst'" := (dmbst cd).
+    Notation "'dmbsy'" := (dmbsy cd).
+    Notation "'dmbld'" := (dmbld cd).
+    Notation "'dsb'" := (dsb cd).
+    Notation "'dsbsy'" := (dsbsy cd).
+
+    Notation "'id'" := ⦗valid_eids cd⦘.
+
+    Definition valid_eids_rc r := r ∪ id.
+    Definition valid_eids_compl a := (valid_eids cd) ∖ a.
+
+    Notation "a ?" := (valid_eids_rc a) (at level 1, format "a ?") : stdpp_scope.
+    Notation "'~~' a" := (valid_eids_compl a)
+                           (at level 1, format "~~ a") : stdpp_scope.
+
+    (* po orders memory events between instructions *)
+    Definition po := ⦗M ∪ F ∪ C⦘⨾instruction_order⨾⦗M ∪ F ∪ C⦘.
+
+    (* other shared relations *)
+    Definition po_loc := po ∩ loc.
+
+    (* wco orders tlbi and writes *)
+    Definition wco := (generic_co cd).
+    Definition co := ⦗W⦘⨾wco⨾⦗W⦘.
+    Definition coi := co ∩ int.
+    Definition coe := co ∖ coi.
+
+    (* rf orders explicit writes and reads *)
+    Definition rf := ⦗W⦘⨾(generic_rf cd)⨾⦗R⦘.
+    Definition rfi := rf ∩ int.
+    Definition rfe := rf ∖ rfi.
+
+    (* armv9-interface/translation.cat#L35 *)
+    Definition trf := (generic_rf cd) ∖ rf.
+    Definition trfi := trf ∩ int.
+    Definition trfe := trf ∖ trfi.
+
+    (* rf orders explicit reads and writes,
+     is unusual because of the handle of initial writes *)
+    Definition fr := (loc ∩ (W × R)) ∖ (co? ⨾ rf)⁻¹.
+    Definition fri := fr ∩ int.
+    Definition fre := fr ∖ fri.
+
+    (* armv9-interface/translation.cat#L46 *)
+    (* Definition tfr := ((trf⁻¹⨾co) ∖ id ) ∩ overlap_loc. *)
+    (* NOTE: To take initial writes under consideration, we have another
+       impelemtation for tfr *)
+    Definition tfr := (overlap_loc ∩ (W × T)) ∖ (co?⨾ rf)⁻¹.
+    Definition tfri := tfr ∩ int.
+    Definition tfre := tfr ∖ tfr.
+
+    #[local] Hint Extern 10 (Decision (?x _)) => unfold x : typeclass_instances.
+    #[local] Hint Extern 10 (Decision (?x _ _)) => unfold x : typeclass_instances.
+    #[local] Hint Extern 10 (Decision (?x _ _ _)) => unfold x : typeclass_instances.
+
+    (*** TLBI *)
+    (* armv9-interface/tlbi.cat *)
+
+    (**  operation *)
+    Definition has_tlb_op_P (P : _ -> Prop) `{forall op, Decision (P op)}
+      (event : iEvent) :=
+      match event with
+      | TlbOp _ op &→ _ => P op
+      | _ => False
+      end.
+
+    Global Instance has_tlb_op_P_dec P `{forall op, Decision (P op)} event :
+      Decision (has_tlb_op_P P event).
+    Proof.  apply _. Qed.
+
+    Definition is_tlbi_op  (tlbiop : TLBIOp) (tlbop : SailArmInstTypes.TLBI) :=
+      tlbop.(TLBI_rec).(TLBIRecord_op) = tlbiop.
+
+    Definition has_tlbi_op (event : iEvent) (tlbiop : TLBIOp) :=
+      has_tlb_op_P (is_tlbi_op tlbiop) event.
+
+    (* armv9-interface/tlbi.cat#L82 *)
+    Definition TLBI_ASID :=
+      collect_all (λ _ event, has_tlbi_op event TLBIOp_ASID
+                              ∨ has_tlbi_op event TLBIOp_VA
+                              ∨ has_tlbi_op event TLBIOp_VAA) cd.
+    (* armv9-interface/tlbi.cat#L89 *)
+    Definition TLBI_S1 :=
+      collect_all (λ _ event, has_tlbi_op event TLBIOp_VA
+                              ∨ has_tlbi_op event TLBIOp_VMALLS12
+                              ∨ has_tlbi_op event TLBIOp_VMALL
+                              ∨ has_tlbi_op event TLBIOp_ALL
+                              ∨ has_tlbi_op event TLBIOp_ASID) cd.
+    (* armv9-interface/tlbi.cat#L98 *)
+    Definition TLBI_S2 :=
+      collect_all (λ _ event, has_tlbi_op event TLBIOp_IPAS2
+                              ∨ has_tlbi_op event TLBIOp_VMALLS12
+                              ∨ has_tlbi_op event TLBIOp_VMALL
+                              ∨ has_tlbi_op event TLBIOp_ALL
+                              ∨ has_tlbi_op event TLBIOp_ASID) cd.
+    (* armv9-interface/tlbi.cat#L108 *)
+    Definition TLBI_VMID :=
+      collect_all (λ _ event, has_tlbi_op event TLBIOp_VA
+                              ∨ has_tlbi_op event TLBIOp_VAA
+                              ∨ has_tlbi_op event TLBIOp_IPAS2
+                              ∨ has_tlbi_op event TLBIOp_VMALLS12
+                              ∨ has_tlbi_op event TLBIOp_VMALL
+                              ∨ has_tlbi_op event TLBIOp_ASID) cd.
+    (* armv9-interface/tlbi.cat#L118 *)
+    Definition TLBI_VA :=
+      collect_all (λ _ event, has_tlbi_op event TLBIOp_VA) cd.
+    (* armv9-interface/tlbi.cat#L121 *)
+    Definition TLBI_IPA :=
+      collect_all (λ _ event, has_tlbi_op event TLBIOp_IPAS2) cd.
+
+    (** regime *)
+    Definition is_tlbi_regime (reg : Regime) (tlbop : SailArmInstTypes.TLBI) :=
+      tlbop.(TLBI_rec).(TLBIRecord_regime) = reg.
+
+    Definition has_tlbi_regime (event : iEvent) (reg : Regime) :=
+      has_tlb_op_P (is_tlbi_regime reg) event.
+
+    (* armv9-interface/tlbi.cat#L126 *)
+    Definition TLBI_EL1 :=
+      collect_all (λ _ event, has_tlbi_regime event Regime_EL10) cd.
+    (* armv9-interface/tlbi.cat#L129 *)
+    Definition TLBI_EL2 :=
+      collect_all (λ _ event, has_tlbi_regime event Regime_EL2) cd.
+
+    (** shareability *)
+    Definition is_tlbi_shareability (share : Shareability)
+      (tlbop : SailArmInstTypes.TLBI) :=
+      tlbop.(TLBI_shareability) = share.
+
+    Definition has_tlbi_shareability (event : iEvent) (share : Shareability) :=
+      has_tlb_op_P (is_tlbi_shareability share) event.
+
+    (* armv9-interface/tlbi.cat#L135 *)
+    Definition TLBI_IS :=
+      collect_all (λ _ event, has_tlbi_shareability event Shareability_ISH
+                              ∨ has_tlbi_shareability event Shareability_OSH) cd.
+
+    (* armv9-interface/tlbi.cat#L142 *)
+    (* This relation is supposed to group [T]s with in the same TTW together,
+     which is not definable with the current outcome interface.
+     We define it as [same_instruction] for now which is only correct if one
+     instruction invokes at most one TTW.
+     *)
+    Definition same_translation : grel EID.t := same_instruction cd.
+
+    Definition get_vmid (event : iEvent) :=
+      match event with
+      | TlbOp _ tlbop &→ _ => Some (tlbop.(TLBI_rec).(TLBIRecord_vmid))
+      | MemRead _ rreq &→ _ => (rreq.(ReadReq.translation).(TranslationInfo_vmid))
+      | _ => None
+      end.
+
+    (* symmetry relation for [T] and [TLBI] with same vmid *)
+    Definition same_vmid := sym_rel_with_same_key cd (λ _ event, get_vmid event).
+
+    Definition get_asid (event : iEvent) :=
+      match event with
+      | TlbOp _ tlbop &→ _ => Some (tlbop.(TLBI_rec).(TLBIRecord_asid))
+      | MemRead _ rreq &→ _ => (rreq.(ReadReq.translation).(TranslationInfo_asid))
+      | _ => None
+      end.
+
+    (* symmetry relation for [T] and [TLBI] with same asid *)
+    Definition same_asid := sym_rel_with_same_key cd (λ _ event, get_asid event).
+
+    (* armv9-interface/tlbi.cat#L158 *)
+    (* NOTE: the definition diverges from the hacky cat version *)
+    Definition tlbi_translate_same_asid : grel EID.t :=
+      (TLBI_ASID × T) ∩ same_asid.
+
+    (* armv9-interface/tlbi.cat#L157 *)
+    (* NOTE: similar to [tlbi_translatr_same_asid] *)
+    Definition tlbi_translate_same_vmid : grel EID.t :=
+      (TLBI_VMID × T) ∩ same_vmid.
+
+    Definition page_of_addr (ad: bits 64): bits 36 := bv_extract 12 36 ad.
+
+    (* below are specialised version of [page_overlaps] *)
+    (* armv9-interface/tlbi.cat#L170 *)
+
+    Definition get_va_page (event : iEvent) :=
+      match event with
+      | MemRead _ rreq &→ _ => match (rreq.(ReadReq.va)) with
+                                    | Some va => Some (page_of_addr va)
+                                    | None => None
+                                    end
+      | TlbOp _ tlbop &→ _ => Some (page_of_addr (tlbop.(TLBI_rec)
+                                                       .(TLBIRecord_address)))
+      | _ => None
+      end.
+
+    Definition va_page_overlap :=
+      sym_rel_with_same_key cd (λ _ event, get_va_page event).
+
+    Definition get_ipa_page (event : iEvent) :=
+      match event with
+      | MemRead _ rreq &→ _ =>
+          match (rreq.(ReadReq.translation).(TranslationInfo_s2info)) with
+          | Some (ipa, _) => Some (page_of_addr ipa)
+          | None => None
+          end
+      | TlbOp _ tlbop &→ _ => Some (page_of_addr
+                                           (tlbop.(TLBI_rec).(TLBIRecord_address)))
+      | _ => None
+      end.
+
+    Definition ipa_page_overlap :=
+      sym_rel_with_same_key cd (λ _ event, get_ipa_page event).
+
+    (* armv9-interface/tlbi.cat#L173 *)
+    Definition tlbi_translate_same_va_page : grel EID.t :=
+      (TLBI_VA × T) ∩ va_page_overlap.
+
+    (* armv9-interface/tlbi.cat#L176 *)
+    Definition tlbi_translate_same_ipa_page : grel EID.t :=
+      (TLBI_IPA × T) ∩ ipa_page_overlap.
+
+    (*** exceptions *)
+    (* armv9-interface/exceptions.cat *)
+
+    (* A Fault is an exception with a FaultRecord *)
+    Definition has_fault_P P `{forall f, Decision (P f)} (event : iEvent) :=
+      match event with
+      | TakeException exn &→ _ => match (exn : Exn).(Exn_fault) with
+                                       | Some fault => P fault
+                                       | _ => False
+                                       end
+      | _ => False
+      end.
+
+    Global Instance has_fault_P_dec P `{forall f, Decision (P f)} event :
+      Decision (has_fault_P P event).
+    Proof. apply _. Qed.
+
+    (* armv9-interface/exceptions.cat#L84 *)
+    Definition Fault := collect_all (λ _ event, has_fault_P (λ _, True) event) cd.
+    (* armv9-interface/exceptions.cat#L94 *)
+    Definition Fault_T :=
+      collect_all
+        (λ _ event,
+           has_fault_P
+             (λ fault, fault.(FaultRecord_statuscode) = Fault_Translation) event) cd.
+    (* armv9-interface/exceptions.cat#L95 *)
+    Definition Fault_P :=
+      collect_all
+        (λ _ event,
+           has_fault_P
+             (λ fault, fault.(FaultRecord_statuscode) = Fault_Permission) event) cd.
+    (* armv9-interface/exceptions.cat#L97 *)
+    Definition FaultFromR :=
+      collect_all
+        (λ _ event,
+           has_fault_P (λ fault, fault.(FaultRecord_write) = false) event) cd.
+    (* armv9-interface/exceptions.cat#L97 *)
+    Definition FaultFromW :=
+      collect_all
+        (λ _ event,
+           has_fault_P (λ fault, fault.(FaultRecord_write) = true) event) cd.
+    (* armv9-interface/exceptions.cat#L103 *)
+    Definition FaultFromAquireR :=
+      collect_all
+        (λ _ event,
+           has_fault_P
+             (λ fault, fault.(FaultRecord_write) = false
+                       ∧ fault.(FaultRecord_acctype) = AccType_ORDERED) event) cd.
+    (* armv9-interface/exceptions.cat#L106 *)
+    Definition FaultFromReleaseW :=
+      collect_all
+        (λ _ event,
+           has_fault_P
+             (λ fault, fault.(FaultRecord_write) = true
+                       ∧ fault.(FaultRecord_acctype) = AccType_ORDERED) event) cd.
+
+    (*** translation-common *)
+    Definition has_translationinfo_P P `{forall ti, Decision (P ti)} (event : iEvent) :=
+      match event with
+      | MemRead _ rreq &→ _ => P (rreq.(ReadReq.translation))
+      | _ => False
+      end.
+
+    Definition is_translationinfo_vmid (vmid : bits 16)
+      (translationinfo: TranslationInfo) :=
+      translationinfo.(TranslationInfo_vmid) = Some vmid.
+    Global Instance is_translationinfo_vmid_dec vmid translationinfo :
+      Decision (is_translationinfo_vmid vmid translationinfo).
+    Proof. apply _. Qed.
+
+    Definition has_translationinfo_vmid (event : iEvent) (vmid : bits 16) :=
+      has_translationinfo_P (is_translationinfo_vmid vmid) event.
+
+    Definition is_translationinfo_asid (asid : bits 16)
+      (translationinfo: TranslationInfo) :=
+      translationinfo.(TranslationInfo_asid) = Some asid.
+    Global Instance is_translationinfo_asid_dec asid translationinfo :
+      Decision (is_translationinfo_asid asid translationinfo).
+    Proof. apply _. Qed.
+
+    Definition has_translationinfo_asid (event : iEvent) (asid : bits 16) :=
+      has_translationinfo_P (is_translationinfo_asid asid) event.
+
+    Definition is_translationinfo_stage1 (translationinfo: TranslationInfo) :=
+      translationinfo.(TranslationInfo_s2info) = None.
+
+    Definition has_translationinfo_stage1 (event : iEvent) :=
+      has_translationinfo_P is_translationinfo_stage1 event.
+    Global Instance has_translationinfo_stage1_dec event :
+      Decision (has_translationinfo_stage1 event).
+    Proof. apply _. Qed.
+
+    (* translation-common.cat#L13 *)
+    Definition Stage1 := collect_all
+                           (λ _ event, is_translate event
+                                       ∧ has_translationinfo_stage1 event) cd.
+
+    Definition is_translationinfo_stage2 (translationinfo: TranslationInfo) :=
+      translationinfo.(TranslationInfo_s2info) ≠ None.
+
+    Definition has_translationinfo_stage2 (event : iEvent) :=
+      has_translationinfo_P is_translationinfo_stage2 event.
+    Global Instance has_translationinfo_stage2_dec event :
+      Decision (has_translationinfo_stage2 event).
+    Proof. apply _. Qed.
+
+    (* translation-common.cat#L14 *)
+    Definition Stage2 := collect_all
+                           (λ _ event, is_translate event
+                                       ∧ has_translationinfo_stage2 event) cd.
+    (* translation-common.cat#L31 *)
+    Definition speculative := ctrl ∪ (addr⨾po) ∪ (⦗T⦘⨾instruction_order).
+    (* translation-common.cat#L37 *)
+    Definition po_pa := (instruction_order ∪ iio) ∩ loc.
+    (* translation-common.cat#L42 *)
+    Definition ContextChange := MSR ∪ TE ∪ ERET.
+    (* translation-common.cat#L46 *)
+    Definition CSE := ISB ∪ TE ∪ ERET.
+
+    (* translation-common.cat#L55 *)
+    Definition tlb_might_affect :=
+      (⦗TLBI_S1 ∩  ~~TLBI_S2 ∩ TLBI_VA ∩ TLBI_ASID⦘⨾
+         (tlbi_translate_same_va_page ∩ tlbi_translate_same_asid
+            ∩ tlbi_translate_same_vmid)⨾⦗T ∩ Stage1⦘)
+        ∪ (⦗TLBI_S1 ∩ ~~TLBI_S2 ∩ TLBI_VA  ∩ TLBI_ASID ∩ ~~TLBI_VMID⦘
+             ⨾(tlbi_translate_same_va_page ∩ tlbi_translate_same_asid)⨾⦗T ∩ Stage1⦘)
+        ∪ (⦗TLBI_S1 ∩ ~~TLBI_S2 ∩ ~~TLBI_VA ∩ TLBI_ASID ∩ TLBI_VMID⦘
+             ⨾(tlbi_translate_same_asid ∩ tlbi_translate_same_vmid)⨾⦗T ∩ Stage1⦘)
+        ∪ (⦗TLBI_S1 ∩ ~~TLBI_S2 ∩ ~~TLBI_VA ∩ ~~TLBI_ASID ∩ TLBI_VMID⦘
+             ⨾tlbi_translate_same_vmid⨾⦗T ∩ Stage1⦘)
+        ∪ (⦗~~TLBI_S1 ∩ TLBI_S2 ∩ TLBI_IPA ∩ ~~TLBI_ASID ∩ TLBI_VMID⦘
+             ⨾(tlbi_translate_same_ipa_page ∩ tlbi_translate_same_vmid)⨾⦗T ∩ Stage2⦘)
+        ∪ (⦗~~TLBI_S1 ∩ TLBI_S2 ∩ ~~TLBI_IPA ∩ ~~TLBI_ASID ∩ TLBI_VMID⦘⨾
+             tlbi_translate_same_vmid⨾⦗T ∩ Stage2⦘)
+        ∪ (⦗TLBI_S1 ∩ TLBI_S2 ∩ ~~TLBI_IPA ∩ ~~TLBI_ASID ∩ TLBI_VMID⦘⨾
+             tlbi_translate_same_vmid⨾⦗T⦘)
+        ∪ (TLBI_S1 ∩ ~~TLBI_IPA ∩ ~~TLBI_ASID ∩ ~~TLBI_VMID) × (T ∩ Stage1)
+        ∪ (TLBI_S2 ∩ ~~TLBI_IPA ∩ ~~TLBI_ASID ∩ ~~TLBI_VMID) × (T ∩ Stage2).
+
+    (* translation-common.cat#L67 *)
+    Definition tlb_affects :=
+      (⦗TLBI_IS⦘⨾tlb_might_affect)
+        ∪ (⦗~~TLBI_IS⦘⨾tlb_might_affect) ∩ int.
+
+    (* translation-common.cat#L75 *)
+    Definition maybe_TLB_cached :=
+      ((⦗T⦘⨾trf⁻¹⨾wco⨾⦗TLBI_S1⦘) ∪
+      (* NOTE: The above line exists because of initial writes are not actual events.
+         Therefore we need to consider T reading from initial writes, and
+       TLBI that are only wco after initial writes separately *)
+         ((T ∖ grel_rng trf) × (TLBI_S1 ∩ (grel_dom wco ∖ grel_rng wco)))
+      ) ∩ tlb_affects⁻¹.
+
+    (* translation-common.cat#L79 *)
+    Definition tob :=
+      (⦗T_f⦘⨾tfr) ∪ (speculative⨾trfi).
+
+    (* translation-common.cat#L85 *)
+    Definition tlb_barriered :=
+      (⦗T⦘⨾tfr⨾wco⨾⦗TLBI⦘) ∩ tlb_affects⁻¹.
+
+    (* translation-common.cat#L88 *)
+    Definition obtlbi_translate :=
+      (* A S1 translation must read from TLB/memory before the TLBI which
+       * invalidates that entry happens *)
+      (⦗T ∩ Stage1⦘⨾tlb_barriered⨾⦗TLBI_S1⦘)
+        (* if the S2 translation is ordered before some S2 write
+         * then the S1 translation has to be ordered before the subsequent
+         * S1 invalidate which would force the S2 write to be visible
+         *
+         * this applies to S2 translations during a S1 walk as well
+         * here the Stage2 translation is only complete once the TLBI VA which
+         * invalidates previous translation-table-walks have been complete *)
+        (* if the S1 translation is from after the TLBI VA
+         * then the S2 translation is only ordered after the TLBI IPA
+         *)
+        ∪ ((⦗T ∩ Stage2⦘⨾tlb_barriered⨾⦗TLBI_S2⦘)
+             ∩ (same_translation⨾⦗T ∩ Stage1⦘⨾trf⁻¹⨾wco⁻¹))
+        (* if the S1 translation is from before the TLBI VA,
+         * then the S2 translation is ordered after the TLBI VA
+         *)
+        ∪ (((⦗T ∩ Stage2⦘⨾tlb_barriered⨾⦗TLBI_S2⦘)⨾(wco ?)⨾⦗TLBI_S1⦘)
+             ∩ (same_translation⨾⦗T ∩ Stage1⦘⨾maybe_TLB_cached)).
+
+    (* translation-common.cat#L110 *)
+    Definition obtlbi :=
+      obtlbi_translate
+        (*
+         * a TLBI ensures all instructions that use the old translation
+         * and their respective memory events
+         * are ordered before the TLBI.
+         *)
+        ∪ (⦗R ∪ W ∪ Fault⦘⨾iio⁻¹⨾(obtlbi_translate ∖ int)⨾⦗TLBI⦘).
+
+    (* translation-common.cat#L123 *)
+    (* context-change ordered-before *)
+    (* note that this is under-approximate and future work is needed
+     * on exceptions and context-changing operations in general *)
+    Definition ctxob :=
+      (* no speculating past context-changing operations *)
+      (speculative⨾⦗MSR⦘)
+        (* context-synchronization orders everything po-after with the
+         synchronization point *)
+        ∪ (⦗CSE⦘⨾instruction_order)
+        (* context-synchronization acts as a barrier for context-changing operations *)
+        ∪ (⦗ContextChange⦘⨾po⨾⦗CSE⦘)
+        (* context-synchronization-events cannot happen speculatively *)
+        ∪ (speculative⨾⦗CSE⦘).
+
+    (* translation-common.cat#L134 *)
+    (* ordered-before a translation fault *)
+    Definition obfault :=
+      data⨾⦗Fault_T ∩ FaultFromW⦘
+        ∪ speculative⨾⦗Fault_T ∩ FaultFromW⦘
+        ∪ ⦗dmbst⦘⨾po⨾⦗Fault_T ∩ FaultFromW⦘
+        ∪ ⦗dmbld⦘⨾po⨾⦗Fault_T ∩ (FaultFromW  ∪ FaultFromR)⦘
+        ∪ ⦗A ∪ Q⦘⨾po⨾⦗Fault_T ∩ (FaultFromW  ∪ FaultFromR)⦘
+        ∪ ⦗R ∪ W⦘⨾po⨾⦗Fault_T ∩ FaultFromW ∩ FaultFromReleaseW⦘.
+
+    (* translation-common.cat#L150 *)
+    (* ETS-ordered-before *)
+    (* if FEAT_ETS then if E1 is ordered-before some Fault
+     then E1 is ordered-before the translation-table-walk read which generated
+     that fault (but not *every* read from the walk, only the one that directly
+     led to the translation fault) Additionally, if ETS then TLBIs are guaranteed
+     completed after DSBs hence po-later translations must be ordered after the
+     TLBI (D5.10.2)
+     *)
+    Definition obETS :=
+      ((obfault⨾⦗Fault_T⦘)⨾iio⁻¹⨾⦗T_f⦘)
+        ∪ ((⦗TLBI⦘⨾po⨾⦗dsb⦘⨾instruction_order⨾⦗T⦘) ∩ tlb_affects).
+
+    (* aarch64_mmu_strong_ETS.cat#L7 *)
+    Definition obs  := rfe ∪ fr ∪ wco ∪ trfe.
+
+    (* aarch64_mmu_strong_ETS.cat#L14 *)
+    Definition dob :=
+      addr ∪ data
+        ∪ (speculative⨾⦗W⦘)
+        ∪ (addr⨾po⨾⦗W⦘)
+        ∪ ((addr ∪ data)⨾rfi)
+        ∪ ((addr ∪ data)⨾trfi).
+
+    (* aarch64_mmu_strong_ETS.cat#L22 *)
+    Definition aob :=
+      rmw
+        ∪ (⦗grel_rng rmw⦘⨾rfi⨾(⦗A⦘∪⦗Q⦘)).
+
+    (* aarch64_mmu_strong_ETS.cat#L26 *)
+    Definition bob :=
+      (⦗R⦘⨾po⨾⦗dmbld⦘)
+        ∪ (⦗W⦘⨾po⨾⦗dmbst⦘)
+        ∪ (⦗dmbst⦘⨾po⨾⦗W⦘)
+        ∪ (⦗dmbld⦘⨾po⨾⦗R ∪ W⦘)
+        ∪ (⦗L⦘⨾po⨾⦗A⦘)
+        ∪ (⦗A ∪ Q⦘⨾po⨾⦗R ∪ W⦘)
+        ∪ (⦗R ∪ W⦘⨾po⨾⦗L⦘)
+        ∪ (⦗F ∪ C⦘⨾po⨾⦗dsbsy⦘)
+        ∪ (⦗dsb⦘⨾po).
+
+    (* aarch64_mmu_strong_ETS.cat#L37 *)
+    (* Ordered-before *)
+    Definition ob1 := obs ∪ dob ∪ aob ∪ bob  ∪ iio ∪ tob ∪ obtlbi ∪ ctxob
+                        ∪ obfault ∪ obETS.
+    (* aarch64_mmu_strong_ETS.cat#L38 *)
+    Definition ob := ob1⁺.
+
+    Record consistent := {
+        (* aarch64_mmu_strong_ETS.cat#L41 *)
+        internal : grel_acyclic (po_loc ∪ fr ∪ co ∪ rf);
+        (* aarch64_mmu_strong_ETS.cat#L44 *)
+        external : grel_irreflexive ob;
+        (* aarch64_mmu_strong_ETS.cat#L47 *)
+        atomic : (rmw ∩ (fre⨾ coe)) = ∅;
+        (* aarch64_mmu_strong_ETS.cat#L50 *)
+        translation_internal : (grel_acyclic (po_pa ∪ trfi));
+      }.
+
+  End def.
+
+  Section wf.
+    Context {nmth : nat}.
+    Context `(cd : Candidate.t nmth).
+    Context `(init_mem : memoryMap).
+    Notation "'rf'" := (rf cd).
+    Notation "'trf'" := (trf cd).
+    Notation "'W'" := (W cd).
+    Notation "'R'" := (R cd).
+    Notation "'A'" := (A cd).
+    Notation "'Q'" := (Q cd).
+    Notation "'L'" := (L cd).
+    Notation "'T'" := (T cd).
+    Notation "'F'" := (F cd).
+    Notation "'C'" := (C cd).
+    Notation "'wco'" := (wco cd).
+    Notation "'ctrl'" := (Candidate.ctrl cd).
+    Notation "'po'" := (po cd).
+
+    Record rf_wf' := {
+        rf_dom : grel_dom rf ⊆ W;
+        rf_rng : grel_rng rf ⊆ R;
+        rf_generic :> NMSWF.generic_rf_wf' cd;
+      }.
+
+    Record trf_wf' := {
+        trf_dom : grel_dom trf ⊆ W;
+        trf_rng : grel_rng trf ⊆ T;
+        trf_generic :> NMSWF.generic_rf_wf' cd;
+      }.
+
+    Record initial_wf' :=
+      {
+        (* reads from initial memory get correct values *)
+        initial_rf : (R ∪ T) ∖ ((grel_rng rf) ∪ (grel_rng trf))
+                     = Candidate.collect_all
+                         (λ eid event, eid ∈ (R ∪ T) ∖ (grel_rng rf)
+                                       ∧ GenArm.is_initial event init_mem) cd;
+      }.
+
+    (* armv9-interface/wco.cat *)
+    Record wco_wf' :=
+      {
+        wco_dom : grel_dom wco ⊆ W ∪ C;
+        wco_rng : grel_rng wco ⊆ W ∪ C;
+        wco_asym : wco ∩ wco⁻¹ = ∅;
+        wco_total : wco ∪ wco⁻¹ = (W ∪ C) × (W ∪ C);
+        wco_w_to_c : wco ∪ wco⁻¹ ⊆ W × C;
+        wco_generic :> NMSWF.generic_co_wf' cd;
+      }.
+
+    Global Instance is_cacheop_dec event : Decision (is_cacheop event).
+    Proof. unfold is_cacheop. apply _. Qed.
+
+    Record event_wf' :=
+      {
+        no_cache_op :=
+          Candidate.collect_all
+            (λ _ event, is_cacheop event) cd = ∅;
+      }.
+
+    Record ctrl_wf' := {
+        ctrl_po : ctrl ⨾ po ⊆ ctrl;
+      }.
+
+    Record wf := {
+        rf_wf :> rf_wf';
+        wco_wf :> wco_wf';
+        initial_wf :> initial_wf';
+        ctrl_wf : ctrl_wf';
+        event_wf :> event_wf';
+      }.
+
+  End wf.
+
+End VMSA.
+
+(*** User *)
+Module UM.
+  Section def.
+    Context {nmth : nat}.
+    Context (cd : Candidate.t nmth).
+    Import Candidate.
+
+    Notation "'rmw'" := (rmw cd).
+    Notation "'addr'" := (addr cd).
+    Notation "'data'" := (data cd).
+    Notation "'ctrl'" := (ctrl cd).
+    Notation "'W'" := (W cd).
+    Notation "'R'" := (R cd).
+    Notation "'M'" := (W ∪ R).
+    Notation "'A'" := (A cd).
+    Notation "'Q'" := (Q cd).
+    Notation "'L'" := (L cd).
+    Notation "'C'" := (C cd).
+    Notation "'int'" := (int cd).
+    Notation "'loc'" := (loc cd).
+
+    Notation "'iio'" := (iio cd).
+    Notation "'instruction_order'" := (instruction_order cd).
+
+    Notation "'dmbst'" := (dmbst cd).
+    Notation "'dmbsy'" := (dmbsy cd).
+    Notation "'dmbld'" := (dmbld cd).
+    Notation "'dsb'" := (dsb cd).
+    Notation "'dsbsy'" := (dsbsy cd).
+    Notation "'ISB'" := (isb cd).
+
+    (* po orders memory events between instructions *)
+    Definition po := ⦗M⦘⨾instruction_order⨾⦗M⦘.
+
+    (* other shared relations *)
+    Definition po_loc := po ∩ loc.
+
+    Definition co := ⦗W⦘⨾(generic_co cd)⨾⦗W⦘.
+    Definition coi := co ∩ int.
+    Definition coe := co ∖ coi.
+
+    (* rf orders explicit writes and reads *)
+    Definition rf := ⦗W⦘⨾(generic_rf cd)⨾⦗R⦘.
+    Definition rfi := rf ∩ int.
+    Definition rfe := rf ∖ rfi.
+
+    Notation "'id'" := ⦗valid_eids cd⦘.
+
+    Definition valid_eids_rc r := r ∪ id.
+    Definition valid_eids_compl a := (valid_eids cd) ∖ a.
+
+    Notation "a ?" := (valid_eids_rc a) (at level 1, format "a ?") : stdpp_scope.
+
+    (* rf orders explicit reads and writes,
+     is unusual because of the handle of initial writes *)
+    Definition fr := (loc ∩ (W × R)) ∖ (co? ⨾ rf)⁻¹.
+    Definition fri := fr ∩ int.
+    Definition fre := fr ∖ fri.
+
+    Definition obs := rfe ∪ fr ∪ co.
+
+    Definition dob :=
+      addr ∪ data
+        ∪ (ctrl⨾⦗W⦘)
+        (* NOTE: (ctrl | addr;po) ; [ISB]; po; [R] is splitted into two,
+         which seems important for one case of the refinement proof *)
+        ∪ ((ctrl ∪ (addr⨾po))⨾⦗ISB⦘)
+        ∪ (⦗ISB⦘⨾po⨾⦗R⦘)
+        ∪ (addr⨾po⨾⦗W⦘)
+        ∪ ((addr ∪ data)⨾rfi).
+
+    Definition aob :=
+      rmw
+        ∪ (⦗grel_rng rmw⦘⨾rfi⨾ (⦗A⦘∪⦗Q⦘)).
+
+    Definition bob :=
+      (⦗R⦘⨾po⨾⦗dmbld⦘)
+        ∪ (⦗W⦘⨾po⨾⦗dmbst⦘)
+        ∪ (⦗dmbst⦘⨾po⨾⦗W⦘)
+        ∪ (⦗dmbld⦘⨾po⨾⦗R ∪ W⦘)
+        ∪ (⦗L⦘⨾po⨾⦗A⦘)
+        ∪ (⦗A ∪ Q⦘⨾po⨾⦗R ∪ W⦘)
+        ∪ (⦗R ∪ W⦘⨾po⨾⦗L⦘)
+        ∪ (⦗dsb⦘⨾ po).
+
+    (* Ordered-before *)
+    Definition ob1 := obs ∪ dob ∪ aob ∪ bob.
+    Definition ob := ob1⁺.
+
+    Record consistent := {
+        internal : grel_acyclic (po_loc ∪ fr ∪ co ∪ rf);
+        external : grel_irreflexive ob;
+        atomic : (rmw ∩ (fre⨾ coe)) = ∅;
+      }.
+
+  End def.
+
+  Section wf.
+    Context {nmth : nat}.
+    Context `(cd : Candidate.t nmth).
+    Context `(init_mem : memoryMap).
+    Notation "'rf'" := (rf cd).
+    Notation "'co'" := (co cd).
+    Notation "'W'" := (W cd).
+    Notation "'R'" := (R cd).
+    Notation "'A'" := (A cd).
+    Notation "'Q'" := (Q cd).
+    Notation "'L'" := (L cd).
+    Notation "'ctrl'" := (Candidate.ctrl cd).
+    Notation "'po'" := (po cd).
+
+    Record rf_wf' := {
+        rf_dom : grel_dom rf ⊆ W;
+        rf_rng : grel_rng rf ⊆ R;
+        rf_generic :> NMSWF.generic_rf_wf' cd;
+      }.
+
+    Record initial_wf' :=
+      {
+        (* reads from initial memory get correct values *)
+        initial_rf : R ∖ (grel_rng rf)
+                     = Candidate.collect_all
+                         (λ eid event, eid ∈ R ∖ (grel_rng rf)
+                                       ∧ GenArm.is_initial event init_mem) cd;
+      }.
+
+    Record co_wf' :=
+      {
+        co_dom : grel_dom co ⊆ W;
+        co_rng : grel_rng co ⊆ W;
+        co_asym : co ∩ co⁻¹ = ∅;
+        co_total : co ∪ co⁻¹ = W × W;
+        co_generic :> NMSWF.generic_co_wf' cd;
+      }.
+
+    Record ctrl_wf' := {
+        ctrl_po : ctrl ⨾ po ⊆ ctrl;
+      }.
+
+    Record event_wf' :=
+      {
+        no_cache_op :=
+          Candidate.collect_all
+            (λ _ event, is_cacheop event) cd = ∅;
+        no_tlbi :=
+          Candidate.collect_all
+            (λ _ event, is_tlbi event) cd = ∅;
+        no_ttw :=
+          Candidate.collect_all
+            (λ _ event, is_translate event) cd = ∅;
+        no_exn :=
+          Candidate.collect_all
+            (λ _ event, is_take_exception event) cd = ∅;
+        no_eret :=
+          Candidate.collect_all
+            (λ _ event, is_return_exception event) cd = ∅;
+        no_msr :=
+          Candidate.collect_all
+            (λ _ event, is_msr event) cd = ∅;
+      }.
+
+    Record wf := {
+        rf_wf :> rf_wf';
+        co_wf :> co_wf';
+        ctrl_wf :> ctrl_wf';
+        initial_wf :> initial_wf';
+        event_wf :> event_wf';
+      }.
+  End wf.
+
+End UM.
