AxiomaticModels/VMUMEquivThm.v
@@ -1,0 +1,804 @@
+Require Import Strings.String.
+
+From stdpp Require Import decidable.
+
+Require Import SSCCommon.Common.
+Require Import SSCCommon.GRel.
+Require Import SSCCommon.FMon.
+Require Import ISASem.ArmInst.
+Require Import ISASem.SailArmInstTypes.
+Require Import GenModels.TermModels.
+Module ArmTM := TermModels Arm.
+Require Import GenModels.CandidateExecutions.
+Module ArmCand := CandidateExecutions Arm ArmTM.
+Require Import GenAxiomaticArm.
+
+Import Arm.
+Import ArmTM.
+Import ArmCand.
+
+Module Thm2.
+
+  Import Candidate.
+
+  (* Given the initial memory [: memoryMap], the root [: pa] of the page table,
+     the range of the page table [: gset pa], this predicate checks that the
+     content of the page table agrees with a characterisation function [: va -> pa] *)
+  (* NOTE: this function is axiomatised for now, since it is not the main goal
+     of this exercise *)
+  Axiom page_table_agree_with_translate : memoryMap -> pa -> gset pa ->
+                                          (va -> pa) -> Prop.
+
+  (* This predicate is an substitution of the translate function in the paper proof *)
+  Axiom translate_read_chain_agree_with_translate : ∀ nmth, Candidate.t nmth -> (va -> pa) -> Prop.
+
+  (* A candidate generated from a full ISA *)
+  Definition cd := GenAxiomaticArm.GenArm.cd.
+  (* the initial memory *)
+  Definition init_mem := GenAxiomaticArm.GenArm.init_mem.
+  (* The candidate is wellformed *)
+  Context (Hwf : GenArm.wellformed cd).
+  (* this is the mathematical characterisation of the page table *)
+  Context (translate : va -> pa).
+  Context (translate_is_inj : FinFun.Injective translate).
+  (* the address space of page table in the initial memory *)
+  Context (page_table_init_address_space : gset (pa)).
+  (* the page table root *)
+  Context (page_table_root : pa).
+  (* the address space of the program *)
+  Context (vm_address_space : gset va).
+
+  (** Hypotheses of the theorems *)
+  (* the two address spaces don't overlap in physical memory *)
+  Context (page_table_vm_pa_disjoint :
+            set_Forall (λ va, translate va ∉ page_table_init_address_space)
+              vm_address_space).
+
+  (** Definition 1 VA abstraction subcondition *)
+  (* NOTE: we do filtering on candidate instead of programs for now, later a
+     similar checker for the associated program should be implemented (by
+     inspecting the initial instruction memory), and a ISA lemma showing
+     that if the program has no such page table affecting instructions then
+     so do its candidates need to be proved. But again, that is not the goal
+     of this exercise *)
+  Definition no_page_table_affecting_events {n} (cd : Candidate.t n) :=
+    (TLBI cd) ∪ (VMSA.ContextChange cd) = ∅.
+
+  (* Check if the page table is static by checking the existence of page table
+     write events (to the initial page table memory) in candidates. Again, we
+     should have a similar check on instructions *)
+  Definition is_page_table_write (event : iEvent) :=
+    match event with
+    | MemWrite _ wreq &→ _ =>
+        wreq.(WriteReq.pa) ∈ page_table_init_address_space
+    | _ => False
+    end.
+  Global Instance is_page_table_write_dec event
+    : Decision (is_page_table_write event).
+  Proof. unfold is_page_table_write. apply _. Qed.
+
+  (* NOTE: this definition might be not very useful in the proof. We might want
+   to first use another def stating that all Ts read from inital memory and later
+   show this def implies that *)
+  Definition page_table_is_static {n} (cd : Candidate.t n) :=
+    collect_all (λ _ event, is_page_table_write event) cd = ∅.
+
+  (** Definition 2 VA abstraction condition *)
+  Definition page_table_is_injective_static {n} (cd : Candidate.t n) :=
+    (* subcondition *)
+    no_page_table_affecting_events cd ∧
+    (* translation function is [translate] which is injective *)
+    page_table_agree_with_translate init_mem page_table_root
+      page_table_init_address_space translate ∧
+    (* and is static *)
+    page_table_is_static cd.
+
+  (* NOTE: The erase function is identity for now since
+    (a) the user model currently is defined by ignoring events - we only show
+    that a full candidate with translation events etc. ignored is consistent with
+    the user model, as the first step;
+    (b) we don't prove properties related to ISAs, esp. after erasure the candidate
+    is a candidate generated with a simplified ISA (without translation), since
+    the ISAs are not ready yet.*)
+  Definition erased_cd := cd.
+
+  Definition thm2_statement :=
+    VMSA.consistent cd ->
+    (* NOTE: Because of the reasons of erasure being identity, we don't need any
+       assumptions on the page table to prove this direction *)
+    (* page_table_is_injective_static -> *)
+    UM.consistent erased_cd.
+
+  (* TODO: we also need to show VMSA.wf cd -> UM.wf cd *)
+
+  (* TODO: move to GRel.v *)
+  Lemma grel_plus_subseteq `{Countable K} (r1 r2 : grel K):
+    r1 ⊆ r2 -> r1⁺ ⊆ r2⁺.
+  Proof.
+    intros Hsub [? ?] Hin.
+    cinduction Hin.
+    - apply Hsub in H0. apply grel_plus_once. assumption.
+    - apply Hsub in H0. eapply grel_plus_trans.
+      + apply grel_plus_once. eassumption.
+      + assumption.
+  Qed.
+
+  (* XXX: the original proof starts by assuming that [addr] in VMSA coincides
+     with [addr] in UM, which is not stated explicitly anywhere in this Coq
+     formalisation. Since here we simply share [addr] between two models, which
+     might not be strictly correct for VMSA?? *)
+  Lemma thm2_proof : thm2_statement.
+  Proof.
+    intros Hvm_cs. destruct Hvm_cs.
+    assert (UM.po erased_cd ⊆ VMSA.po cd) as Hpo.
+    {
+      unfold UM.po, VMSA.po. clear.
+      Local Typeclasses Opaque W R F C loc instruction_order.
+      set_unfold. hauto lq:on.
+      Local Typeclasses Transparent W R F C loc instruction_order.
+    }
+    Local Typeclasses Opaque UM.po VMSA.po.
+    split.
+    - assert (UM.po_loc erased_cd ⊆ VMSA.po_loc cd).
+      {
+        unfold UM.po_loc, VMSA.po_loc.
+        clear - Hpo.
+        set_solver + Hpo.
+      }
+      Local Typeclasses Opaque UM.po_loc VMSA.po_loc.
+      assert (UM.fr erased_cd = VMSA.fr cd) as ->.
+      {
+        clear. set_unfold. done.
+      }
+      assert (UM.co erased_cd = VMSA.co cd) as ->.
+      {
+        clear. set_unfold. done.
+      }
+      assert (UM.rf erased_cd = VMSA.rf cd) as ->.
+      {
+        clear. set_unfold. done.
+      }
+      clear - internal H.
+      Local Typeclasses Opaque VMSA.rf VMSA.fr VMSA.co.
+      assert (UM.po_loc erased_cd ∪ VMSA.fr cd ∪ VMSA.co cd ∪ VMSA.rf cd
+        ⊆ VMSA.po_loc cd ∪ VMSA.fr cd ∪ VMSA.co cd ∪ VMSA.rf cd).
+      set_solver + H.
+      clear H. apply grel_plus_subseteq in H0.
+      set_solver.
+      Local Typeclasses Transparent VMSA.rf VMSA.fr VMSA.co.
+    - assert (UM.ob erased_cd ⊆ VMSA.ob cd) as Hincl.
+      {
+        clear internal atomic translation_internal.
+        unfold UM.ob, VMSA.ob. apply grel_plus_subseteq.
+        unfold UM.ob1, VMSA.ob1.
+        assert (UM.obs erased_cd ⊆ VMSA.obs cd) as Hobs.
+        {
+          unfold UM.obs, VMSA.obs.
+          assert (UM.co erased_cd ⊆ VMSA.wco cd).
+          {
+            set_unfold; hauto.
+          }
+          clear external. set_unfold; sauto lq:on.
+        }
+        assert (UM.dob erased_cd ⊆ VMSA.dob cd ∪ VMSA.ctxob cd) as Hdob.
+        {
+          unfold UM.dob, VMSA.dob.
+          assert (ctrl erased_cd ⨾ ⦗W erased_cd⦘ ⊆ VMSA.speculative cd ⨾ ⦗W cd⦘)
+            as Hdob.
+          {
+            unfold VMSA.speculative. clear Hobs external.
+            set_unfold. hauto lq: on rew: off.
+          }
+          clear -Hdob Hpo.
+          assert ((ctrl erased_cd ∪ addr erased_cd ⨾ UM.po erased_cd) ⨾ ⦗isb erased_cd⦘
+                    ∪ ⦗isb erased_cd⦘ ⨾ UM.po erased_cd ⨾ ⦗R erased_cd⦘ ⊆ VMSA.ctxob cd) as Hctxob.
+          {
+            unfold VMSA.ctxob.
+            apply union_subseteq. split.
+            - clear - Hpo.
+              assert (ctrl erased_cd ∪ (addr erased_cd ⨾ UM.po erased_cd)
+                        ⊆  VMSA.speculative cd).
+              {
+                unfold VMSA.speculative.
+                hauto lq:on simp+:set_unfold.
+              }
+              unfold VMSA.CSE. set_unfold. hauto lq:on.
+            - transitivity (⦗VMSA.CSE cd⦘ ⨾ instruction_order cd).
+              + assert ( UM.po erased_cd ⨾ ⦗R erased_cd⦘ ⊆ instruction_order cd).
+                {
+                  clear - Hpo.
+                  unfold UM.po. set_solver.
+                }
+                clear -H.
+                Local Typeclasses Opaque isb UM.po R instruction_order.
+                unfold VMSA.CSE. set_solver.
+                Local Typeclasses Transparent isb UM.po R instruction_order.
+              + Local Typeclasses Opaque VMSA.CSE instruction_order VMSA.speculative MSR VMSA.ContextChange.
+                set_solver.
+                Local Typeclasses Transparent VMSA.CSE instruction_order VMSA.speculative MSR VMSA.ContextChange.
+          }
+          Local Typeclasses Opaque VMSA.CSE VMSA.speculative VMSA.ctxob W R isb UM.po VMSA.trfi VMSA.po.
+          set_unfold. hauto lq: on rew: off.
+          Local Typeclasses Transparent VMSA.CSE VMSA.speculative VMSA.ctxob W R isb UM.po VMSA.trfi VMSA.po.
+        }
+        assert (UM.aob erased_cd ⊆ VMSA.aob cd) as Haob.
+        {
+          set_solver +.
+        }
+        assert (UM.bob erased_cd ⊆ VMSA.bob cd) as Hbob.
+        {
+          unfold UM.bob, VMSA.bob.
+          clear - Hpo.
+          Local Typeclasses Opaque  W R L A Q dmbld dmbst dmbsy dsb dsbsy isb UM.po VMSA.po.
+          set_unfold. hauto lq: on rew: off.
+          Local Typeclasses Transparent W R L A Q dmbld dmbst dmbsy dsb dsbsy isb UM.po VMSA.po.
+        }
+        clear external.
+        (* make definitions opaque to avoid unnecessary unfolding *)
+        Local Typeclasses Opaque UM.obs VMSA.obs UM.dob VMSA.dob UM.aob VMSA.aob
+          UM.bob VMSA.bob VMSA.tob VMSA.obtlbi VMSA.ctxob VMSA.obfault VMSA.obETS.
+        set_unfold. sauto lq:on.
+      }
+      set_solver + Hincl external.
+    - assumption.
+  Admitted.
+
+  (* Definition 4 translation extension *)
+  (* NOTE: we omit this step for now, just assuming that the VMSA candidate cd
+     is obtained after the extension, then we write down the charactorisations of
+     the extension (correspond to the 5 extension items) as some assumptions below.
+   *)
+  Definition translation_extension_cd := cd.
+
+  (* Point 1: Instead of adding initial writes, we assume all page table writes
+     are initial writes, namely no page table writes except for initial writes,
+     or page table is static *)
+  Definition translation_extension_initial_writes {n} (cd : Candidate.t n) :=
+    page_table_is_static cd.
+
+  (* Immediate iio *)
+  Definition iio_imm {n} (cd : Candidate.t n) := iio cd ∖ (iio cd ⨾ iio cd).
+
+  (* Point 2,3, and 5: Instead of adding translation reads, we assume all translate
+     reads read from initial page table writes (which is derivable from WF), whose
+     charactorisation is the translate function; and instead of inserting translate
+     reads, we assume each memory access is immediately iio ordered-before the
+     chain of proper translate reads *)
+  (* NOTE the translate function is not the one in the paper proof *)
+  Record translation_extension_translate_reads {n} (cd : Candidate.t n) := {
+      (* the trf is empty, this means Ts only read from initial writes (given WF) *)
+      trf_empty: grel_rng (VMSA.trf cd) = ∅;
+      (* all Ts read from page table address space *)
+      T_rf_init: collect_all
+                   (λ _ event, is_translate event
+                               ∧ match get_pa event with
+                                 | Some pa => pa ∈ page_table_init_address_space
+                                 | _ => False
+                                 end) cd
+                 = T cd;
+      (* page table's charactorisation is translate *)
+      page_table_is_translate : page_table_agree_with_translate init_mem
+                                  page_table_root
+                                  page_table_init_address_space translate;
+      (* no translate reads that cause translation fault *)
+      no_T_f : T_f cd = ∅ ;
+      (* this is a quite strong assumption, but should be fine for this exercise *)
+      no_MSR : MSR cd = ∅ ;
+      (* all Ts that are supposed to be added to the user candidate by translation
+       extensions are in a chain of form [T];same_translation;[T];...imm(iio);[M] *)
+      T_in_chain :
+      T cd = grel_dom(⦗T cd⦘
+                         ⨾(((VMSA.same_translation cd)∩ iio_imm cd)⨾⦗T cd⦘)⁺
+                         ⨾iio_imm cd⨾⦗W cd ∪ R cd⦘);
+      (* TODO: more conditions TBA, unclear for now *)
+      T_correct_in_cd : translate_read_chain_agree_with_translate n cd translate
+    }.
+
+  (* NOTE: Point 4 needs no charactorisation, since we assume addr coincides *)
+
+  (* Definition 5: VA anti anstraction condition *)
+  (* NOTE: just a conjunction *)
+  Definition translation_events_and_relations_are_simple_and_nice {n} (cd : Candidate.t n) :=
+    translation_extension_initial_writes cd
+    ∧ translation_extension_translate_reads cd
+    ∧ no_page_table_affecting_events cd
+    ∧ UM.consistent cd.
+
+  (* Lemma 1 VA abstraction condition for translation extension *)
+  (* NOTE: we are cheating here since we don't have extension. So we simply check
+     if we are missing any conditions *)
+  Definition conditions_sanity_check :
+    translation_events_and_relations_are_simple_and_nice translation_extension_cd ->
+    page_table_is_injective_static translation_extension_cd.
+  Proof.
+    intros (?&?&?&?). destruct H0.
+    split; first assumption.
+    split; assumption.
+  Qed.
+
+  Section obtlbi_empty.
+
+  Lemma obtlbi_empty n (cd : Candidate.t n) :
+    translation_events_and_relations_are_simple_and_nice cd ->
+    VMSA.obtlbi cd = ∅.
+  Proof.
+    intros (?&?&?&?).
+    clear - H1.
+    unfold VMSA.obtlbi.
+    assert (VMSA.obtlbi_translate cd = ∅).
+    {
+      unfold VMSA.obtlbi_translate.
+      Local Typeclasses Opaque T VMSA.Stage1 VMSA.tlb_barriered
+      VMSA.maybe_TLB_cached VMSA.trf VMSA.same_translation.
+      assert (TLBI cd = ∅). set_unfold; sauto lq:on. clear H1.
+      assert (VMSA.TLBI_S1 cd = ∅).
+      {
+        Local Typeclasses Opaque VMSA.is_tlbi_op.
+        set_unfold.
+        (* FIXME: hauto & sauto are very slow *)
+        unfold is_tlbi in H.
+        intros ? [? [? ?]]. apply (H x).
+        eexists. split; first eassumption.
+        unfold VMSA.has_tlbi_op. unfold VMSA.has_tlb_op_P. hauto.
+      }
+      assert (VMSA.TLBI_S2 cd = ∅).
+      {
+        set_unfold.
+        unfold is_tlbi in H.
+        intros ? [? [? ?]]. apply (H x).
+        eexists. split; first eassumption.
+        unfold VMSA.has_tlbi_op. unfold VMSA.has_tlb_op_P. hauto.
+      }
+        Local Typeclasses Opaque VMSA.TLBI_S1 VMSA.TLBI_S2.
+      set_unfold. hauto lq: on.
+    }
+    assert (⦗R cd ∪ W cd ∪ VMSA.Fault cd⦘ ⨾ (iio cd) ⁻¹
+              ⨾ VMSA.obtlbi_translate cd ∖ int cd ⨾ ⦗TLBI cd⦘ = ∅).
+    {
+      Local Typeclasses Opaque VMSA.Fault VMSA.obtlbi_translate R W int.
+      set_unfold. sauto lq:on.
+    }
+    set_unfold. hauto lq:on.
+  Qed.
+  End obtlbi_empty.
+
+  Section po_pa_W_trf_empty.
+
+    (* Lemma 3 the proof is easier than paper version, due to our treatment of
+     initial writes *)
+  Lemma po_pa_W_trf_empty {n} (cd : Candidate.t n) :
+    GenArm.wellformed cd ->
+    translation_events_and_relations_are_simple_and_nice cd ->
+    grel_acyclic (VMSA.po_pa cd ∪ VMSA.trfi cd).
+  Proof.
+    intros Hwf (?&?&?&?). destruct H0.
+    clear -trf_empty0 Hwf.
+    assert (VMSA.trfi cd = ∅) as ->.
+    {
+      clear - trf_empty0.
+      Local Typeclasses Opaque VMSA.trf.
+      unfold VMSA.trfi.
+      set_unfold. hauto.
+    }
+    clear trf_empty0. unfold VMSA.po_pa.
+    destruct Hwf. destruct generic_po0.
+    apply grel_transitive_rew in generic_po_trans.
+    clear -generic_po_irr generic_po_trans.
+    set_unfold.
+    intros ? Hin.
+    assert ((instruction_order cd ∪ iio cd) ∩ loc cd ⊆ generic_po cd) as Hsub.
+    {
+      clear. unfold iio, instruction_order.
+      set_unfold. sauto.
+    }
+    apply grel_plus_subseteq in Hsub.
+    rewrite union_empty_r_L in Hin.
+    apply Hsub in Hin. rewrite generic_po_trans in Hin.
+    eapply generic_po_irr. eassumption.
+  Qed.
+
+  End po_pa_W_trf_empty.
+
+  Section ob_to_T.
+    (* TODO: it is unclear how to state it properly at this moment, so skip *)
+    Lemma ob_to_T {n} (cd : Candidate.t n):
+      translation_events_and_relations_are_simple_and_nice cd ->
+      VMSA.ob cd ⨾⦗T cd⦘
+      = iio cd.
+    Proof. Admitted.
+  End ob_to_T.
+
+  Section no_cycle_ob_to_init.
+    (* Lemma 5 *)
+    (* NOTE: we don't really need this lemma, neither can state it because of
+     our treatment of initial writes *)
+    Lemma no_cycle_ob_to_init : True.
+    Proof. done. Qed.
+  End no_cycle_ob_to_init.
+
+  (* TODO: move to GRel.v *)
+  (* things about grel_seq *)
+  Lemma grel_seq_union_r `{Countable K} (r1 r2 r2' : grel K):
+    r1 ⨾ (r2 ∪ r2') = (r1 ⨾ r2) ∪ (r1 ⨾ r2').
+  Proof.
+    set_unfold. hauto lq:on.
+  Qed.
+
+  Lemma grel_seq_union_l `{Countable K} (r1 r1' r2 : grel K):
+    (r1 ∪ r1') ⨾ r2 = (r1 ⨾ r2) ∪ (r1' ⨾ r2).
+  Proof.
+    set_unfold. hauto lq:on.
+  Qed.
+
+  Global Instance grel_seq_assoc `{Countable K}: Assoc (=) ( (@grel_seq K _ _) ).
+  Proof.
+    intros ??. set_unfold. hauto lq:on.
+  Qed.
+
+  Section ob_from_T.
+
+    Definition M {n} (cd : Candidate.t n) :=
+      collect_all (λ _ event, is_mem_event event) cd.
+
+    (* NOTE: the paper version of this lemma is wrong:
+       it doesn't have the last case ([T];instruction-order;[ISB]) on the RHS *)
+    Lemma ob_from_T {n} (cd : Candidate.t n) :
+      translation_events_and_relations_are_simple_and_nice cd ->
+      GenArm.wellformed cd ->
+      (* We simply assume the extended candidate is wf wrt VMSA, but this is a
+       property about the extension that we want to show *)
+      VMSA.wf cd init_mem ->
+      ⦗T cd⦘⨾VMSA.ob1 cd =
+      iio cd
+        ∪ (⦗T cd⦘⨾iio cd ⨾⦗M cd⦘⨾ VMSA.po cd ⨾⦗W cd⦘)
+        ∪ (⦗T cd⦘⨾ instruction_order cd ⨾ ⦗isb cd⦘).
+    Proof.
+      intros (?&?&?&?) Hwf Hvmsa_wf. unfold VMSA.ob1.
+      (* general proof strategy: check all clauses of ob1 *)
+      unfold VMSA.obs.
+      assert (T cd ## W cd) as H_T_W_disj.
+      {
+        (* FIXME: seemed hauto is not smart enough for things like it *)
+        clear. set_unfold. unfold is_translate, is_mem_write.
+        intros ? (?&Hlk1&?) (?&Hlk2&?).
+        rewrite Hlk1 in Hlk2.
+        hauto lq: on rew: off.
+      }
+      assert (T cd ## C cd) as H_T_C_disj.
+      {
+        clear. set_unfold. unfold is_translate, is_mem_read.
+        intros ? (?&Hlk1&?) (?&Hlk2&?).
+        rewrite Hlk1 in Hlk2.
+        hauto lq: on rew: off.
+      }
+      assert (T cd ## R cd) as H_T_R_disj.
+      {
+        clear. set_unfold. unfold is_translate, is_mem_read.
+        intros ? (?&Hlk1&?) (?&Hlk2&?).
+        unfold is_explicit_access_kind_P in H0.
+        rewrite Hlk1 in Hlk2; inversion Hlk2; subst.
+        destruct x1 as [T call ret]. destruct call;try assumption. rewrite H in H0.
+        hauto lq:on.
+      }
+      assert (⦗T cd⦘⨾ (VMSA.rfe cd) = ∅).
+      {
+        unfold VMSA.rfe. unfold VMSA.rf. clear - H_T_W_disj.
+        Local Typeclasses Opaque VMSA.rfi R T W.
+        set_unfold. sauto lq:on.
+        Local Typeclasses Transparent VMSA.rfi R T W.
+      }
+      assert (⦗T cd⦘⨾ (VMSA.fr cd) = ∅).
+      {
+        unfold VMSA.fr. clear - H_T_W_disj.
+        Local Typeclasses Opaque VMSA.co VMSA.rf T W.
+        set_unfold. sauto lq:on.
+        Local Typeclasses Transparent VMSA.co VMSA.rf R T W.
+      }
+      assert (⦗T cd⦘⨾ (VMSA.wco cd) = ∅).
+      {
+        destruct Hvmsa_wf. clear - wco_wf H_T_C_disj H_T_W_disj.
+        destruct wco_wf. clear -H_T_C_disj H_T_W_disj wco_dom.
+        set_unfold. ecrush lq: on.
+      }
+      assert (⦗T cd⦘⨾ (VMSA.trfe cd) = ∅).
+      {
+        unfold VMSA.trfe. destruct H0. clear -trf_empty0.
+        Local Typeclasses Opaque VMSA.trfi T.
+        set_unfold. sauto lq:on.
+        Local Typeclasses Transparent VMSA.trfi T.
+      }
+      assert (⦗T cd⦘⨾ (VMSA.dob cd)
+              = ⦗T cd⦘ ⨾ instruction_order cd ⨾ ⦗W cd⦘).
+      {
+        unfold VMSA.dob.
+        assert (⦗T cd⦘⨾ (addr cd) = ∅).
+        {
+          destruct Hwf. destruct addr0. clear - addr_dom H_T_R_disj.
+          Local Typeclasses Opaque T R.
+          set_unfold. sauto lq: on rew: off.
+          Local Typeclasses Transparent T R.
+        }
+        assert (⦗T cd⦘⨾ (data cd) = ∅).
+        {
+          destruct Hwf. destruct data0. clear - data_dom H_T_R_disj.
+          Local Typeclasses Opaque T R.
+          set_unfold. sauto lq: on rew: off.
+          Local Typeclasses Transparent T R.
+        }
+        assert (⦗T cd⦘⨾ (ctrl cd) = ∅).
+        {
+          destruct Hwf. destruct ctrl0. clear - ctrl_dom H_T_R_disj.
+          Local Typeclasses Opaque T R.
+          set_unfold. sauto lq: on rew: off.
+          Local Typeclasses Transparent T R.
+        }
+        assert (⦗T cd⦘ ⨾ addr cd ⨾ VMSA.po cd = ∅ ).
+        {
+          Local Typeclasses Opaque VMSA.po addr T.
+          clear -H7.
+          set_unfold.
+          intros ? (?&?&?). apply (H7 (x.1, x0)). simpl. assumption.
+          Local Typeclasses Transparent VMSA.po addr T.
+        }
+        assert (⦗T cd⦘⨾ (addr cd ⨾ VMSA.po cd ⨾ ⦗W cd⦘) = ∅).
+        {
+          clear -H10.
+          rewrite assoc. 2: apply _.
+          Local Typeclasses Opaque T addr VMSA.po.
+          set_unfold. sauto lq: on rew: off.
+          Local Typeclasses Transparent T addr VMSA.po.
+        }
+        assert (⦗T cd⦘⨾ (VMSA.speculative cd ⨾ ⦗W cd⦘)
+                = ⦗T cd⦘ ⨾ instruction_order cd ⨾⦗W cd⦘).
+        (* TODO: We further need to use [T_in_chain] to show that there must be a
+         iio ordered after [M] before [W] *)
+        {
+          unfold VMSA.speculative.
+          Local Typeclasses Opaque T W instruction_order ctrl data addr VMSA.po.
+          clear - H10 H9.
+          rewrite assoc. 2: apply _.
+          assert (⦗T cd⦘ ⨾ (ctrl cd ∪ addr cd ⨾ VMSA.po cd) = ∅ ).
+          {
+            set_unfold. hauto lq:on.
+          }
+          clear H9.
+          set_unfold. hauto lq: on.
+          Local Typeclasses Transparent T W instruction_order ctrl data addr VMSA.po.
+        }
+        assert (⦗T cd⦘⨾ ((addr cd ∪ data cd) ⨾ VMSA.rfi cd) = ∅).
+        {
+          clear - H7 H8.
+          Local Typeclasses Opaque T W instruction_order data addr VMSA.po VMSA.rfi.
+          rewrite assoc. 2: apply _.
+          set_unfold.
+          intros ? (?&?&?). destruct H as (? & ?& [? |?]).
+          apply (H7 (x1, x0)). hauto l:on.
+          apply (H8 (x1, x0)). hauto l:on.
+          Local Typeclasses Transparent T W instruction_order data addr VMSA.po VMSA.rfi.
+        }
+        assert (⦗T cd⦘⨾ ((addr cd ∪ data cd) ⨾ VMSA.trfi cd) = ∅).
+        {
+          clear - H7 H8.
+          Local Typeclasses Opaque T W instruction_order data addr VMSA.po VMSA.rfi.
+          rewrite assoc. 2: apply _.
+          set_unfold.
+          intros ? (?&?&?). destruct H as (? & ?& [? |?]).
+          apply (H7 (x1, x0)). hauto l:on.
+          apply (H8 (x1, x0)). hauto l:on.
+          Local Typeclasses Transparent T W instruction_order data addr VMSA.po VMSA.rfi.
+        }
+        clear -H7 H8 H9 H11 H12 H13 H14.
+        Local Typeclasses Opaque T W data addr ctrl VMSA.speculative VMSA.rfi VMSA.trfi instruction_order VMSA.po.
+        repeat rewrite grel_seq_union_r.
+        rewrite H7, H8, H11, H12, H13, H14.
+        clear.
+        set_unfold. hauto lq:on.
+        Local Typeclasses Transparent T W data addr ctrl VMSA.speculative VMSA.rfi VMSA.trfi instruction_order VMSA.po.
+      }
+      assert (⦗T cd⦘⨾ (VMSA.aob cd) = ∅).
+      {
+        unfold VMSA.aob.
+        (* FIXME need WF lxsx amo, easy *)
+        admit.
+      }
+      assert (⦗T cd⦘⨾ (VMSA.bob cd) = ∅).
+      {
+        unfold VMSA.bob.
+        clear - H_T_W_disj H_T_C_disj H_T_R_disj.
+        assert (T cd ## L cd) as H_T_L_disj.
+        {
+          clear. set_unfold. unfold is_translate, is_mem_read.
+          intros ? (?&Hlk1&?) (?&Hlk2&?).
+          rewrite Hlk1 in Hlk2.
+          hauto rew:off lq:on.
+        }
+        assert (T cd ## Q cd) as H_T_Q_disj.
+        {
+          clear. set_unfold. unfold is_translate, is_mem_read.
+          intros ? (?&Hlk1&?) (?&Hlk2&?).
+          rewrite Hlk1 in Hlk2; inversion Hlk2; subst.
+          destruct x1 as [T call ret]. unfold is_explicit_access_kind_P in H0.
+          destruct call;try assumption. rewrite H in H0.
+          hauto lq:on.
+        }
+        assert (T cd ## A cd) as H_T_A_disj.
+        {
+          clear. set_unfold. unfold is_translate, is_mem_read.
+          intros ? (?&Hlk1&?) (?&Hlk2&?).
+          rewrite Hlk1 in Hlk2; inversion Hlk2; subst.
+          destruct x1 as [T call ret]. unfold is_explicit_access_kind_P in H0.
+          destruct call;try assumption. rewrite H in H0.
+          hauto lq:on.
+        }
+        assert (T cd ## F cd) as H_T_F_disj.
+        {
+          clear. set_unfold. unfold is_translate, is_mem_read.
+          intros ? (?&Hlk1&?) (?&Hlk2&?).
+          rewrite Hlk1 in Hlk2.
+          hauto rew:off lq:on.
+        }
+        assert (T cd ## dmbst cd) as H_T_dmbst_disj.
+        {
+          clear. set_unfold. unfold is_translate, is_mem_read.
+          intros ? (?&Hlk1&?) (?&Hlk2&?).
+          rewrite Hlk1 in Hlk2.
+          hauto rew:off lq:on.
+        }
+        assert (T cd ## dmbld cd) as H_T_dmbld_disj.
+        {
+          clear. set_unfold. unfold is_translate, is_mem_read.
+          intros ? (?&Hlk1&?) (?&Hlk2&?).
+          rewrite Hlk1 in Hlk2.
+          hauto rew:off lq:on.
+        }
+        assert (T cd ## dsb cd) as H_T_dsb_disj.
+        {
+          clear. set_unfold. unfold is_translate, is_mem_read.
+          intros ? (?&Hlk1&?) (?&Hlk2&?).
+          rewrite Hlk1 in Hlk2.
+          hauto rew:off lq:on.
+        }
+        Local Typeclasses Opaque T R W dmbst dmbld L A Q F C dsb dsbsy.
+        set_unfold. ecrush drew: off lq: on.
+        Local Typeclasses Transparent T R W dmbst dmbld L A Q F C dsb dsbsy.
+      }
+      assert (⦗T cd⦘⨾ VMSA.tob cd = ∅).
+      {
+        unfold VMSA.tob.
+        rewrite grel_seq_union_r.
+        do 2 rewrite grel_seq_assoc.
+        destruct H0.
+        rewrite no_T_f0.
+        assert (VMSA.trfi cd = ∅) as ->.
+        {
+          unfold VMSA.trfi. clear -trf_empty0.
+          Local Typeclasses Opaque VMSA.trf int.
+          set_unfold. hauto lq: on.
+          Local Typeclasses Transparent VMSA.trf int.
+        }
+        clear.
+        Local Typeclasses Opaque T VMSA.tfr VMSA.speculative.
+        set_unfold. hauto lq: on.
+        Local Typeclasses Transparent T VMSA.tfr VMSA.speculative.
+      }
+      assert (⦗T cd⦘⨾ VMSA.obtlbi cd = ∅).
+      {
+        unfold VMSA.obtlbi.
+        rewrite grel_seq_union_r.
+        assert (⦗T cd⦘⨾ VMSA.obtlbi_translate cd = ∅) as ->.
+        {
+          unfold VMSA.obtlbi_translate.
+          repeat rewrite grel_seq_union_r.
+          repeat rewrite grel_seq_assoc.
+          assert (⦗VMSA.TLBI_S1 cd⦘ = ∅) as ->.
+          {
+            clear -H1.
+            unfold no_page_table_affecting_events in H1.
+            Local Typeclasses Opaque VMSA.ContextChange.
+            set_unfold.
+            unfold VMSA.has_tlbi_op. unfold VMSA.has_tlb_op_P. unfold is_tlbi in H1.
+            intros ? ([e ?]&Heq). apply (H1 x.1).
+            left.  destruct e as [T call ret]. destruct call; hauto lq:on.
+          }
+          assert (⦗VMSA.TLBI_S2 cd⦘ = ∅) as ->.
+          {
+            clear -H1.
+            unfold no_page_table_affecting_events in H1.
+            set_unfold.
+            unfold VMSA.has_tlbi_op. unfold VMSA.has_tlb_op_P. unfold is_tlbi in H1.
+            intros ? ([e ?]&Heq). apply (H1 x.1).
+            left.  destruct e as [T call ret]. destruct call; hauto lq:on.
+          }
+          Local Typeclasses Opaque T VMSA.Stage1 VMSA.tlb_barriered VMSA.Stage2 VMSA.trf VMSA.wco VMSA.same_translation valid_eids VMSA.maybe_TLB_cached.
+          clear.
+          set_unfold. hauto lq:on.
+          Local Typeclasses Transparent VMSA.ContextChange T VMSA.Stage1 VMSA.tlb_barriered VMSA.Stage2 VMSA.trf VMSA.wco VMSA.same_translation valid_eids VMSA.maybe_TLB_cached.
+        }
+        assert (⦗TLBI cd⦘ = ∅) as ->.
+        {
+        unfold no_page_table_affecting_events in H1.
+        clear -H1. set_unfold. hauto lq:on.
+        }
+        clear.
+        Local Typeclasses Opaque T R W VMSA.Fault iio VMSA.obtlbi_translate int.
+        set_unfold. hauto lq: on.
+        Local Typeclasses Transparent T R W VMSA.Fault iio VMSA.obtlbi_translate int.
+      }
+      assert (⦗T cd⦘⨾ VMSA.ctxob cd =⦗T cd⦘⨾ instruction_order cd ⨾ ⦗isb cd⦘).
+      {
+        unfold VMSA.ctxob.
+        do 2 rewrite grel_seq_union_r.
+        rewrite grel_seq_union_r.
+        assert (⦗T cd⦘⨾ (VMSA.speculative cd ⨾ ⦗VMSA.CSE cd⦘)
+                = ⦗T cd⦘⨾ instruction_order cd ⨾ ⦗isb cd⦘) as -> .
+        {
+          rewrite grel_seq_assoc.
+          (* easy *)
+          admit.
+        }
+        assert (⦗VMSA.ContextChange cd⦘ = ∅) as ->.
+        {
+        unfold no_page_table_affecting_events in H1.
+        clear -H1. set_unfold. hauto lq:on.
+        }
+        assert (⦗MSR cd⦘ = ∅) as ->.
+        {
+          destruct H0. rewrite no_MSR0. done.
+        }
+        assert (⦗T cd⦘ ⨾ (⦗VMSA.CSE cd⦘ ⨾ instruction_order cd) = ∅) as ->.
+        {
+          rewrite grel_seq_assoc. unfold VMSA.CSE.
+          assert (T cd ## isb cd ∪ TE cd ∪ ERET cd) as H_T_disj.
+          {
+            clear. set_unfold. unfold is_translate, is_mem_read.
+            intros ? (?&Hlk1&?) [[(?&Hlk2&?)|(?&Hlk2&?)]|(?&Hlk2&?)];
+            rewrite Hlk1 in Hlk2; hauto rew:on lq:on.
+          }
+          clear -H_T_disj.
+          Local Typeclasses Opaque T isb TE ERET.
+          set_unfold. hauto lq: on.
+          Local Typeclasses Transparent T isb TE ERET.
+        }
+        clear.
+        Local Typeclasses Opaque T VMSA.speculative VMSA.po VMSA.CSE instruction_order.
+        set_unfold. hauto lq: on.
+        Local Typeclasses Transparent T VMSA.speculative VMSA.po VMSA.CSE instruction_order.
+      }
+      assert (⦗T cd⦘⨾ VMSA.obfault cd = ∅).
+      {
+        unfold VMSA.obfault.
+        do 4 rewrite grel_seq_union_r.
+        do 8 rewrite grel_seq_assoc.
+        (* easy *)
+        admit.
+      }
+      assert (⦗T cd⦘⨾ VMSA.obETS cd = ∅).
+      {
+        unfold VMSA.obETS.
+        rewrite grel_seq_union_r.
+        assert (⦗TLBI cd⦘ = ∅) as ->.
+        {
+        unfold no_page_table_affecting_events in H1.
+        clear -H1. set_unfold. hauto lq:on.
+        }
+        do 3 rewrite grel_seq_assoc.
+        rewrite H13.
+        clear.
+        Local Typeclasses Opaque T VMSA.Fault_T iio T_f VMSA.po instruction_order VMSA.tlb_affects.
+        set_unfold. hauto lq: on.
+        Local Typeclasses Transparent T VMSA.Fault_T iio T_f VMSA.po instruction_order VMSA.tlb_affects.
+      }
+    Admitted.
+
+  End ob_from_T.
+
+  (* TODO: incomplete *)
+  Definition thm3_statement :=
+    UM.consistent cd ->
+    page_table_is_injective_static cd ->
+    VMSA.consistent cd.
+
+  Lemma thm3_proof : thm3_statement.
+  Proof. Admitted.
+
+End Thm2.
